proof/Russell/GenerationCoerce.v
@@ -26,13 +26,9 @@ Fixpoint type_range (t : term) : term :=
 
 Definition type_dom (t : term) : term :=
   match t with
-  | Prod U V => type_range U
   | Sum U V => type_range U
-  | Subset U V => type_range U
-  | _ => type_range t
+  | _ => t
   end.
-
-Definition is_low_sort (s : term) := s = Srt set \/ s = Srt prop.
 
 Lemma subst_to_sort : forall t t' s, subst t t' = Srt s -> t <> Srt s ->
   t' = Srt s.
@@ -54,16 +50,32 @@ Proof.
   intros ; discriminate.
 Qed.
 
-Lemma kind_is_prod_aux : forall G t T, G |- t : T -> T = Srt kind ->
-  is_low_sort (type_range t).
+Fixpoint is_low t : Prop :=
+  match t with 
+  | Prod T U => is_low U
+  | Sum U V => is_low U \/ is_low V
+  | Srt s => is_prop s
+  | _ => False
+  end.
+
+Lemma red_sort_eq : forall s t, red (Srt s) t -> t = Srt s.
 Proof.
-  induction 1 ; intros ; try discriminate ; simpl ; auto.
-  unfold is_low_sort ; intuition.
-  unfold is_low_sort ; intuition.
-  induction (wf_sort_lift H H0).
+  simple induction 1; intros; auto with coc core arith sets.
   rewrite H1 in H2.
-  elim (typ_not_kind H2) ; auto.
+  inversion H2.
+Qed.
+
+Lemma kind_is_prod_aux : forall G t T, G |- t : T -> 
+  T = Srt kind -> is_low t.
+Proof.
+  unfold is_prop ; induction 1 ; intros ; try discriminate ; simpl ; auto.
+
+  unfold is_prop ; intuition.
+  unfold is_prop ; intuition.
   
+  induction (wf_sort_lift H H0).
+  elim (typ_not_kind H2) ; auto.
+
   pose (subst_to_sort _ H1 (typ_not_kind H)).
 
   pose (type_no_kind_type H0 (or_introl _ (refl_equal (Prod V Ur)))).
@@ -72,47 +84,42 @@ Proof.
   rewrite e0 in H3.
   simpl in H3.
   contradiction.
+  
+  inversion H2.
+  rewrite H4 in H1.
+  induction H1 ; intuition ; try discriminate.
 
+  rewrite H1 in IHtyp1.
+  intuition.
+  rewrite H1 in IHtyp2 ; intuition.
+  
   pose (type_no_kind_type H (or_intror _ (refl_equal (Sum U V)))).
+  rewrite H0 in t0.
   simpl in t0.
   destruct t0.
-  rewrite H0 in H1.
-  simpl in H1.
   contradiction.
 
+  assert(Pi1 t <> Srt kind).
+  red ; intros ; discriminate.
+  pose (subst_to_sort _ H0 H1).
   pose (type_no_kind_type H (or_intror _ (refl_equal (Sum U V)))).
+  rewrite e0 in t0.
   simpl in t0.
   destruct t0.
-  assert(Pi1 t <> Srt kind) ; try (unfold not ; intros ; discriminate).
-  pose (subst_to_sort _ H0 H3).
-  rewrite e0 in H2.
-  simpl in H2.
   contradiction.
-
-(*  pose (type_has_no_kind H).
-  pose (type_has_no_kind H2).
-  unfold subst in H3.
-  pose (type_range_subst_not_kind _ _ 0 t0 t1).
-  pose (type_no_kind_not_kind t2).
-  contradiction.*)
-
-  rewrite H3 in H0.
-  pose (typ_not_kind H0).
-  elim n ; auto.
+  
+  rewrite H3 in H2.
+  pose (coerce_sort_r H2).
+  elim (typ_not_kind t0).
+  auto.
 Qed.
 
-Lemma type_kind_range : forall G t, G |- t : Srt kind -> is_low_sort (type_range t).
+Lemma type_kind_range : forall G t, G |- t : Srt kind -> is_low t.
 Proof.
   intros.
   apply kind_is_prod_aux with G (Srt kind) ; auto.
 Qed.
 
-Lemma red_sort_eq : forall s t, red (Srt s) t -> t = Srt s.
-Proof.
-  simple induction 1; intros; auto with coc core arith sets.
-  rewrite H1 in H2.
-  inversion H2.
-Qed.
 
 Lemma sort_conv_eq : forall G T s, G |- T : Srt kind -> conv T (Srt s) -> T = Srt s.
 Proof.
@@ -122,7 +129,7 @@ Proof.
   rewrite e in H1.
 
   pose (type_kind_range H).
-  unfold is_low_sort in i.
+  unfold is_low in i.
   induction T ; try (simpl in i ; destruct i ; inversion H1 ; try discriminate) ; auto with coc core.
 
   rewrite (conv_sort _ _ H0).
@@ -130,10 +137,6 @@ Proof.
 
   rewrite (conv_sort _ _ H0).
   auto.
-
-  pose (conv_sort_prod s T1 T2).
-  pose (sym_conv _ _ H0).
-  contradiction.
 
   pose (conv_sort_prod s T1 T2).
   pose (sym_conv _ _ H0).
@@ -231,4 +234,157 @@ Proof.
   apply coerce_propset_r_aux with G (Srt s) s'; auto.
   apply coerce_sort_r_in_kind with G A s ; auto.
 Qed.
+
+Fixpoint no_sort t : Prop :=
+  match t with 
+  | Prod T U => no_sort U
+  | Sum U V => no_sort U /\ no_sort V
+  | Srt s => False
+  | _ => True
+  end.
+
+Fixpoint is_low_full t : Prop :=
+  match t with 
+  | Prod T U => is_low_full U
+  | Sum U V => (is_low_full U /\ is_low_full V) \/ (is_low_full U /\ no_sort V) \/
+  (is_low_full V /\ no_sort U)
+  | Srt s => is_prop s
+  | _ => False
+  end.
+
+Lemma sort_of_kinded_aux : forall G t T, G |- t : T -> 
+  forall s, T = Srt s -> 
+  (s = kind -> is_low_full t) /\ (is_prop s -> no_sort t).
+Proof.
+  unfold is_prop ; induction 1 ; intros ; try discriminate ; simpl ; auto.
+
+  unfold is_prop ; intuition.
+  rewrite H2 in H0 ; discriminate.
+  rewrite H2 in H0 ; discriminate.
+  
+  split ; intros ; unfold is_prop ; auto.
+  intuition ; rewrite H2 in H0 ; discriminate.
+
+  split ; intros.
+  rewrite H2 in H1.
+  induction (wf_sort_lift H H0).
+  rewrite H1 in H3.
+  elim (typ_not_kind H3) ; auto.
+  auto.
+
+  split ; intros ; auto.
+  rewrite H2 in H1.
+  pose (subst_to_sort _ H1 (typ_not_kind H)).
+
+  pose (type_no_kind_type H0 (or_introl _ (refl_equal (Prod V Ur)))).
+  simpl in t.
+  destruct t.
+  rewrite e0 in H4.
+  simpl in H4.
+  contradiction.
+  
+  inversion H2.
+  rewrite H4 in H1.
+  split ; intros.
+  rewrite H3 in H1.
+  induction H1 ; intuition ; try discriminate.
+
+  rewrite H1 in IHtyp1.
+  destruct (IHtyp1 kind) ; auto.
+
+  destruct (IHtyp2 set) ; auto.
+  rewrite H5 ; auto.
+  right ; left ; intuition.
+
+  destruct (IHtyp1 set) ; auto.
+  rewrite H5 ; auto.
+  destruct (IHtyp2 kind) ; auto.
+  rewrite H1 ; auto.
+  right ; right ; intuition.
+
+  destruct H3.
+  rewrite H3 in H1 ; destruct H1 ; intuition ; try discriminate.
+  destruct (IHtyp1 prop) ; auto.
+  rewrite H5 ; auto.
+  destruct (IHtyp2 prop) ; auto.
+  rewrite H1 ; auto.
+  
+  rewrite H3 in H1 ; destruct H1 ; intuition ; try discriminate.
+  destruct (IHtyp1 set) ; auto.
+  rewrite H5 ; auto.
+  destruct (IHtyp2 set) ; auto.
+  rewrite H1 ; auto.
+
+  split ; intros.
+  rewrite H2 in H1 ; discriminate.
+  auto.
+
+  split ; intros.
+  rewrite H1 in H0.
+  
+  pose (type_no_kind_type H (or_intror _ (refl_equal (Sum U V)))).
+  simpl in t0.
+  destruct t0.
+  rewrite H0 in H2.
+  simpl in H2.
+  contradiction.
+  
+  auto.
+
+  split ; intros ; auto.
+  pose (type_no_kind_type H (or_intror _ (refl_equal (Sum U V)))).
+  simpl in t0.
+  destruct t0.
+  assert(Pi1 t <> Srt s).
+  red ; intros ; discriminate.
+  pose (subst_to_sort _ H0 H4).
+  rewrite H1 in e0.
+  rewrite e0 in H3.
+  simpl in H3.
+  contradiction.
+
+  assert(s = kind).
+  pose (coerce_sort_r H2).
+  rewrite H3 in t0.
+  destruct (typ_sort t0).
+  inversion H5.
+  auto.
+
+  destruct (IHtyp3 kind) ; rewrite <- H4 ; auto.
+  destruct (IHtyp2 kind) ; try rewrite <- H4 ; auto.
+  split ; intros.
+  rewrite H4 in H9.
+  rewrite H9 in H3.
+  rewrite H3 in H7.
+  unfold is_low, is_prop in H7 ; simpl in H7.
+  destruct (H7 (refl_equal kind)) ; discriminate.
+
+  clear H6 H5 H7 H8.
+  rewrite H3 in H2.
+  pose (coerce_propset_r H2).
+  destruct (IHtyp1 s0 e0).
+  auto.
+Qed.
+
+Lemma sorts_of_sorted : forall G t s, G |- t : Srt s -> 
+  (s = kind -> is_low_full t) /\ (is_prop s -> no_sort t).
+Proof.
+  intros.
+  apply sort_of_kinded_aux with G (Srt s) ; auto ; auto.
+Qed. 
+
+Lemma sort_of_kinded : forall G t, G |- t : Srt kind -> 
+  is_low_full t.
+Proof.
+  intros ; destruct (sorts_of_sorted H).
+  apply H0 ; auto.
+Qed.
+
+Lemma sort_of_propset : forall G t s, G |- t : Srt s -> 
+  is_prop s -> no_sort t.
+Proof.
+  intros ; destruct (sorts_of_sorted H).
+  apply H2 ; auto.
+Qed.
+
 
