proof/Russell/Types.v
@@ -10,33 +10,15 @@ Implicit Types i k m n p : nat.
 Implicit Type s : sort.
 Implicit Types A B M N T t u v : term.
 
+Reserved Notation "G |- T = U : s" (at level 70, T, U, s at next level).
 Reserved Notation "G |- T >> U : s" (at level 70, T, U, s at next level).
 Reserved Notation "G |- T : U" (at level 70, T, U at next level).
 
-Definition sum_sort U V s1 s2 :=
-  (U = Srt set /\ V = Srt set) \/
-  (s1 = set /\ s2 = set).
-
-
-Lemma sum_sort_lift : forall T U s1 s2, sum_sort T U s1 s2 ->
-  forall n n' k k', sum_sort (lift_rec n T k) (lift_rec n' U k') s1 s2.
-Proof.
-  unfold sum_sort ; intros.
-  destruct H.
-  induction H ; rewrite H ; auto with coc.
-  rewrite H0 ; auto with coc.
-
-  induction H ; rewrite H ; rewrite H0 ; auto with coc.
-Qed.
-
-Lemma sum_sort_subst : forall T U s1 s2, sum_sort T U s1 s2 ->
-  forall t k k', sum_sort (subst_rec t T k) (subst_rec t U k') s1 s2.
-Proof.
-  unfold sum_sort ; intros.
-  destruct H.
-  induction H ; rewrite H ; rewrite H0 ; auto with coc.
-  induction H ; rewrite H ; rewrite H0 ; auto with coc.
-Qed.
+Definition sum_sort s1 s2 s3 :=
+  (s1 = set /\ s2 = set /\ s3 = set) \/
+  (s1 = kind /\ s2 = set /\ s3 = kind) \/
+  (s1 = set /\ s2 = kind /\ s3 = kind) \/
+  (s1 = prop /\ s2 = prop /\ s3 = prop).
 
 Inductive coerce : env -> term -> term -> sort -> Prop :=
   | coerce_refl : forall e A s, e |- A : Srt s -> e |- A >> A : s
@@ -53,8 +35,8 @@ Inductive coerce : env -> term -> term -> sort -> Prop :=
   (* derivable *) e |- A' : Srt s -> e |- A : Srt s ->
   forall s', (A :: e) |- B >> B' : s' ->
   (* derivable *) A :: e |- B : Srt s' -> A' :: e |- B' : Srt s' ->
-  sum_sort A B s s' -> sum_sort A' B' s s' ->
-  e |- (Sum A B) >> (Sum A' B') : s'
+  forall s'', sum_sort s s' s'' -> sum_sort s s' s'' ->
+  e |- (Sum A B) >> (Sum A' B') : s''
 
   | coerce_sub_l : forall e U P U', 
   e |- U >> U' : set ->
@@ -75,6 +57,22 @@ where "G |- T >> U : s" := (coerce G T U s)
 with wf : env -> Prop :=
   | wf_nil : wf nil
   | wf_var : forall e T s, e |- T : (Srt s) -> wf (T :: e)
+
+with convt : env -> term -> term -> sort -> Prop :=
+  | convt_prod : forall e U V U' V' s1 s2, 
+  e |- U = U' : s1 -> U' :: e |- V = V' : s2 ->
+  e |- Prod U V = Prod U' V' : s2
+
+  | convt_sum : forall e U V U' V' s1 s2, 
+  e |- U = U' : s1 -> U :: e |- V = V' : s2 ->
+  e |- Sum U V = Sum U' V' : s2
+
+  | convt_sub : forall e U V U' V' s1 s2, 
+  e |- U = U' : set -> U :: e |- V = V' : prop ->
+  e |- Subset U V = Subset U' V' : s2
+  
+  | convt_conv : forall e U V s, 
+  e |- U : s -> e |- V : s -> conv U V -> e |- U = V : s.
 
 with typ : env -> term -> term -> Prop :=
   | type_prop : forall e, wf e -> e |- (Srt prop) : (Srt kind)
@@ -98,7 +96,7 @@ with typ : env -> term -> term -> Prop :=
     forall u, e |- u : U ->
     forall V s2, (U :: e) |- V : (Srt s2) ->
     forall v, e |- v : (subst u V) -> 
-    sum_sort U V s1 s2 ->
+    forall s3, sum_sort s1 s2 s3 ->
     e |- (Pair (Sum U V) u v) : (Sum U V)
 
   | type_prod :
@@ -113,8 +111,8 @@ with typ : env -> term -> term -> Prop :=
       e |- T : (Srt s1) ->
       forall (U : term) s2,
       (T :: e) |- U : (Srt s2) -> 
-      sum_sort T U s1 s2 ->
-      e |- (Sum T U) : (Srt s2)
+      forall s3, sum_sort s1 s2 s3 ->
+      e |- (Sum T U) : Srt s3
 
   | type_subset : 
       forall e T, e |- T : (Srt set) ->
@@ -122,7 +120,8 @@ with typ : env -> term -> term -> Prop :=
       e |- (Subset T U) : (Srt set)
 
   | type_pi1 :
-      forall e t U V, e |- t : (Sum U V) -> e |- (Pi1 t) : U
+      forall e t U V, e |- t : (Sum U V) -> 
+      e |- (Pi1 t) : U
 
   | type_pi2 :
       forall e t U V, e |- t : (Sum U V) -> 
@@ -244,8 +243,8 @@ Proof.
   induction 1 ; intros ; split ; try (intuition ; intros ; auto with coc core).
   apply type_prod with s ; auto with coc core.
   apply type_prod with s ; auto with coc core.
-  apply type_sum with s ; auto with coc core.
-  apply type_sum with s ; auto with coc core.
+  apply type_sum with s s' ; auto with coc core.
+  apply type_sum with s s' ; auto with coc core.
   apply type_subset ; auto with coc core.
   apply type_subset ; auto with coc core.
 Qed.
