proof/Russell/RussellMinus/Types.v
@@ -1,0 +1,105 @@
+Require Import Termes.
+Require Import LiftSubst.
+Require Import Reduction.
+Require Import Conv.
+Require Import Env.
+
+Set Implicit Arguments.
+
+Implicit Types i k m n p : nat.
+Implicit Type t : sort.
+Implicit Types A B M N T u v : term.
+
+Reserved Notation "G |- T : s" (at level 70, T, s at next level).
+
+Inductive type : Set :=
+  | in_set : type
+  | in_prop : type
+  | star : type
+  | box : type.
+
+Definition interp (s : sort) : type :=
+  match s with
+  | prop => in_prop
+  | set => in_set
+  | kind => star
+  end.
+
+Definition sum_sort' s1 s2 s3 :=
+  (s1 = in_set /\ s2 = in_set /\ s3 = in_set) \/
+  (s1 = star /\ s2 = in_set /\ s3 = star) \/
+  (s1 = in_set /\ s2 = star /\ s3 = star) \/
+  (s1 = in_prop /\ s2 = in_prop /\ s3 = in_prop).
+
+Inductive wf_minus : env -> Prop :=
+  | wf_nil : wf_minus nil
+  | wf_var : forall e T s, e |- T : s -> wf_minus (T :: e)
+
+with typ_minus : env -> term -> type -> Prop :=
+  | type_prop : forall e, wf_minus e -> e |- (Srt prop) : star
+  | type_set : forall e, wf_minus e -> e |- (Srt set) : star
+
+  | type_var : (* start *)
+  forall e, wf_minus e -> forall n T, item_lift T e n ->
+  forall s, e |- T : s -> e |- (Ref n) : s
+
+  | type_abs :
+      forall e T s1,
+      e |- T : s1 ->
+      forall M (U : term) s2,
+      (T :: e) |- U : s2 ->
+      (T :: e) |- M : s2 -> 
+      e |- (Abs T M) : s2
+  | type_app :
+      forall e v s1, e |- v : s1 ->
+      forall u s, e |- u : s -> 
+      e |- (App u v) : s
+
+  | type_pair :
+    forall e (U : term) s1, e |- U : s1 ->
+    forall u su, e |- u : su ->
+    forall V s2, (U :: e) |- V : s2 ->
+    forall v, e |- v : s2 -> 
+    forall s3, sum_sort' s1 s2 s3 ->
+    e |- (Pair (Sum U V) u v) : s3
+
+  | type_prod :
+      forall e T s1,
+      e |- T : s1 ->
+      forall (U : term) s2,
+      (T :: e) |- U : s2 -> 
+      e |- (Prod T U) : s2
+
+  | type_sum :
+      forall e T s1,
+      e |- T : s1 ->
+      forall (U : term) s2,
+      (T :: e) |- U : s2 -> 
+      forall s3, sum_sort' s1 s2 s3 ->
+      e |- (Sum T U) : s3
+
+  | type_subset : 
+      forall e T, e |- T : in_set ->
+      forall (U : term), (T :: e) |- U : in_prop -> 
+      e |- (Subset T U) : in_set
+
+  | type_pi1 :
+      forall e (t : term) s, e |- t : s -> 
+      e |- (Pi1 t) : s
+
+  | type_pi2 :
+      forall e (t : term) s, e |- t : s -> 
+      e |- (Pi2 t) : s
+
+(*  | type_let_in :
+      forall e t U, e |- t : U ->
+      forall s1, e |- U : (Srt s1) -> (* Just for easier induction, derivable from the next 
+	 judgment *)
+      forall v M, (U :: e) |- v : M -> 
+      forall s2, (U :: e) |- M : (Srt s2) ->
+      e |- (Let_in t v) : (subst t M) *)
+
+where "G |- T : U" :=  (typ_minus G T U).
+
+Lemma soundness : forall G t e
+
